

Session 14 Course Title: Mathematics II Course Code: MAT102/0541-102 Credits: 3	Course Teacher: Md. Yousuf Ali (YA) Lecturer, Department of GED. Email: yousufkumath@gmail.com Mobile: 01766906098
--	---

Laplace Equation and Harmonic Function

Laplacian: The second order partial differential operator is called the Laplacian. Mathematically it is defined by

$$\nabla^2 = \frac{\partial^2}{\partial x^2} + \frac{\partial^2}{\partial y^2}.$$

Laplace's Equation in two dimensions: The second order partial differential equation is called the Laplace equation in two dimensions.

Mathematically it is defined by

$$\nabla^2 u = 0 \Rightarrow \frac{\partial^2 u}{\partial x^2} + \frac{\partial^2 u}{\partial y^2} = 0$$

where, $u(x, y)$ is the real valued function.

Harmonic Function: Any function of two variables x and y is said to be harmonic on a domain D , if throughout D it has second order continuous partial derivatives and satisfies the Laplace's equation.

Example: Examine the following function u is harmonic or not, if it is harmonic then **Construct** the conjugate harmonic function v .

$$u(x, y) = 2x + 3xy^2 - x^3$$

Solution: Given that,

$$u(x, y) = 2x + 3xy^2 - x^3 \dots \dots \dots (i)$$

Now partially differentiating (i) with respect to x and y , we get

$$\frac{\partial u}{\partial x} = u_x = \frac{\partial}{\partial x} \{u(x, y)\} = \frac{\partial}{\partial x} (2x + 3xy^2 - x^3) = 2 + 3y^2 - 3x^2 \dots \dots \dots \text{(ii)}$$

$$\frac{\partial u}{\partial y} = u_y = \frac{\partial}{\partial y} \{u(x, y)\} = \frac{\partial}{\partial y} (2x + 3xy^2 - x^3) = 6xy \dots \dots \dots \text{(iii)}$$

Again partially differentiating equation (ii) with respect to x and equation (iii) with respect to y , we get,

$$\frac{\partial^2 u}{\partial x^2} = u_{xx} = \frac{\partial}{\partial x} \left(\frac{\partial u}{\partial x} \right) = \frac{\partial}{\partial x} (2 + 3y^2 - 3x^2) = -6x \dots \dots \dots \text{(iv)}$$

$$\frac{\partial^2 u}{\partial y^2} = u_{yy} = \frac{\partial}{\partial y} \left\{ \frac{\partial u}{\partial y} \right\} = \frac{\partial}{\partial y} (6xy) = 6x \dots \dots \dots \text{(v)}$$

Now by adding equation (iv) and (v), we get

$$\frac{\partial^2 u}{\partial x^2} + \frac{\partial^2 u}{\partial y^2} = -6x + 6x = 0$$

Which satisfies the Laplace's equation so the function is said to be a harmonic function.

For conjugate harmonic:

We have the C-R equation,

$$\frac{\partial u}{\partial x} = \frac{\partial v}{\partial y} \dots \dots \dots \text{(vi)}$$

$$\frac{\partial u}{\partial y} = -\frac{\partial v}{\partial x} \dots \dots \dots \text{(vii)}$$

From (vi), we can write

$$\frac{\partial u}{\partial x} = \frac{\partial v}{\partial y} \Rightarrow \frac{\partial v}{\partial y} = 2 + 3y^2 - 3x^2 \text{ [Using (ii)]}$$

$$\Rightarrow \frac{\partial v}{\partial y} = 2 + 3y^2 - 3x^2$$

$$\Rightarrow \partial v = \int (2 + 3y^2 - 3x^2) \partial y$$

$$\Rightarrow v = 2y + 3\frac{y^3}{3} - 3x^2y + C(x)$$

$$\therefore v = 2y + y^3 - 3x^2y + C(x) \dots \dots \dots \text{(viii)}$$

Partially differentiating equation (viii) w.r.t x , we get

$$\frac{\partial v}{\partial x} = \frac{\partial}{\partial x} \{2y + y^3 - 3x^2y + C(x)\} = -6xy + C'(x) \dots \dots \dots \text{(ix)}$$

From equation (vii)

$$\frac{\partial u}{\partial y} = -\frac{\partial v}{\partial x} \Rightarrow 6xy = -\{-6xy + C'(x)\} \text{ [Using (iii) and (ix)]}$$

$$\Rightarrow 6xy = 6xy - C'(x)$$

$$\Rightarrow C'(x) = 0$$

$$\Rightarrow \frac{dC(x)}{dx} = 0$$

$$\Rightarrow dC(x) = 0$$

$$\therefore C(x) = c \text{ [By integrating]}$$

Thus the conjugate harmonic function of u is

$$\therefore v = 2y + y^3 - 3x^2y + c \text{ (Ans.)}$$

Assignment

1. Examine the following function u is harmonic or not, if it is harmonic then **Construct** the conjugate harmonic function v . Also **Setup** the complex variable $f(z) = u + iv$.

$$\textbf{i.} \quad u(x, y) = 2xy + 3xy^2 - 2y^3 \qquad \textbf{iv.} \quad u(x, y) = xe^x \cos y - ye^x \sin y$$

$$\textbf{ii.} \quad u(x, y) = e^{-x} (x \cos y - y \sin y) \qquad \textbf{v.} \quad u(x, y) = e^{x^2-y^2} \cos 2xy$$

$$\textbf{iii.} \quad u(x, y) = \frac{1}{2} \ln(x^2 + y^2)$$